`Subset` renamed `IsComponent`

Z/Environment.lean
@@ -2,107 +2,97 @@ import Z.Util
 
 /- TODO: remove duplicates?  -/
 
-
 def Environment (R: Type u) := R
 
-infixr:67 " *: " => Prod.mk
+/--
+`IsComponent A B` means that a permutation of `A` is part of `B`.
 
+Symbolic form: A ∣ B.
 
-def t1 := 1 *: "a" *: true
+For example if `A = A₁ × A₂` then 
+```
+A ∣ (B₁ × A₁ × B₂ × A₂)
+A ∣ (A₁ × B₁ × B₂ × A₂)
+A ∣ (A₁ × A₂ × B₁ × B₂)
+A ∣ (A₂ × A₁ × B₁ × B₂)
+... 
+```
+all are valid.
 
+`Unit` is assumed to be part of any product.
 
-/-- Helper type class to extract a value of type A from Env  -/
-
-private class GetElement (Env) (A) where
-  apply: Env -> A
-
-
-/-- Recursive case  -/
-instance [getter: GetElement (Environment T) B] : GetElement (Environment (A × T)) B where
-  apply | (_, t) => getter.apply t
-
-/-- Base case: element is the head  -/
-instance : GetElement (Environment (A × T)) A where
-  apply | (a, _) => a
-
-/-- Special case: just one element  -/
-instance : GetElement (Environment A) A where
-  apply a := a
-
-
-/- -------------  -/
-
-/- TODO: Find a better name -/
-class Subset (A : Type u) (B: Type v) where
+- `get: B -> A` is the projection. 
+-/
+class IsComponent (A : Type u) (B: Type v) where
   get: B -> A
 
-
-infixl:65 " ⊂ " => Subset
-
-def Subset.contramap {C} [inst: A ⊂ B] (f: A -> C): C ⊂ B :=
-  ⟨inst.get ∘> f⟩
+ 
+infixl:65 " ∣ " => IsComponent
 
 
-/-- different tails but head1 is in tail2 and tail1 is subset of tuple2 -/
-instance [H₁ ⊂ T₂] [T₁ ⊂ (H₂ × T₂)] : (H₁ × T₁) ⊂ (H₂ × T₂) where
-  get | (h₂, t₂) => (Subset.get t₂, Subset.get (h₂, t₂))
+namespace IsComponent
 
-/-- Same heads and tail1 is subset of tail2  -/
-instance [T₁ ⊂ T₂] : (H × T₁) ⊂ (H × T₂) where 
-  get | (h, t₂) => (h, Subset.get t₂)
-
-/- Different heads but head1 is subset of tail -/
-instance [H₁ ⊂ T] : H₁ ⊂ (H × T) where
-  get | (_, t) => Subset.get t
-
-/-- A few base cases  -/
-instance : H ⊂ (H × T) := ⟨fun (h, _) => h⟩
-instance : L ⊂ L       := ⟨id⟩
-instance : Unit ⊂ L    := ⟨fun _ => ()⟩
+  def contramap [component: A ∣ B] (f: A -> C): C ∣ B :=
+    ⟨get ∘> f⟩
 
 
-def accept [R1 ⊂ R2] (_: Environment R1) (_: Environment R2) := true
+  /-- 
+  This will detect permutations of `A × B` in `H × T`.
 
-/- rule 0 -/
-example: accept () () = true := rfl
-example: accept () ('c' *: "a" *: 1) = true := rfl
+  If we reach this case then we know that `A ≠ H` (as this is covered by `rule4`).
 
+  So we need to things:
+  - `A` is in `T`
+  - `B` is in `H × T`
 
-/- rule1: same head -/
+  -/
+  instance rule5 [A ∣ T] [B ∣ (H × T)] : (A × B) ∣ (H × T) where
+    get | (h, t) => (get t, get (h, t))
 
--- equal elements
-example: accept 'c' 'c' = true := rfl
-example: accept ("a" *: 1) ("a" *: 1) = true := rfl
-example: accept ('c' *: "a" *: 1) ('c' *: "a" *: 1) = true := rfl
+  /-- Same heads and different tails but one tail is a component of the other -/
+  instance rule4 [B ∣ T] : (A × B) ∣ (A × T) where 
+    get | (a, t) => (a, get t)
 
+  /- Either A is in the head or the tail -/
+  instance rule3 [A ∣ T] : A ∣ (H × T) := ⟨fun (_, t) => get t⟩
+  instance rule2         : A ∣ (A × T) := ⟨fun (a, _) => a⟩
 
--- more elements provided than required
-example: accept 'c' ('c' *: "a" *: 1 *: true) = true := rfl
-example: accept ('c' *: "a" *: 1) ('c' *: "a" *: 1 *: true) = true := rfl
+  /-- A few base cases  -/
+  instance rule1 :    L ∣ L := ⟨id⟩
+  instance rule0 : Unit ∣ L := ⟨fun _ => ()⟩
 
--- negative:
-#check_failure accept ('c' *: "a" *: 1 *: true) ('c' *: "a" *: 1)
+end IsComponent
 
+namespace IsComponentExamples
+  def accept [R1 ∣ R2] (_: Environment R1) (_: Environment R2) := true
 
-/- rule2: -/
-example: accept ("a" *: 1) ('c' *: "a" *: 1) = true := rfl
+  /- Base cases -/
+  example: accept () () = true := rfl
+  example: accept () ('c', "a", 1) = true := rfl
 
-example: accept (1 *: "a") ('c' *: "a" *: 1) = true := rfl
+  /- equal elements -/
+  example: accept 'c' 'c' = true := rfl
+  example: accept ("a", 1) ("a", 1) = true := rfl
+  example: accept ('c', "a", 1) ('c', "a", 1) = true := rfl
 
-example: accept "a" ('c' *: "a" *: 1) = true := rfl
+  /- more elements provided than required -/
+  example: accept 'c' ('c', "a", 1, true) = true := rfl
+  example: accept ('c', "a", 1) ('c', "a", 1, true) = true := rfl
 
-example: accept ("a" *: 'c' *: 1) ('c' *: "a" *: 1) = true := rfl
+  -- negative:
+  #check_failure accept ('c', "a", 1, true) ('c', "a", 1)
 
-#check_failure accept (1 *: "a" *: 'c') (true *: 1)
+  /- Other rules -/
+  example: accept ("a", 1) ('c', "a", 1) = true := rfl
+  example: accept (1, "a") ('c', "a", 1) = true := rfl
+  example: accept "a"      ('c', "a", 1) = true := rfl
+  example: accept ("a", 'c', 1) ('c', "a", 1) = true := rfl
 
-#check_failure accept ('c' *: "a" *: 1) []
+  #check_failure accept (1, "a", 'c') (true, 1)
+  #check_failure accept ('c', "a", 1) []
 
+end IsComponentExamples
 
-
-
-
-
-/- -------------  -/
 
 namespace Environment 
 
@@ -119,8 +109,8 @@ namespace Environment
   def concat (self: Environment T) (ea: Environment A) : Environment (A × T) := 
     ⟨ea, self⟩ 
 
-  def get (self: Environment T) (A) [getter: GetElement (Environment T) A] : A :=
-    getter.apply self
+  def get (self: Environment T) (A) [component: A ∣ T] : A :=
+    component.get self
 
   def of (a: A) : Environment A := 
     empty.add a
@@ -131,20 +121,25 @@ namespace Environment
 
 end Environment 
 
-
--- #check_failure Environment.get [] Char
-
--- #eval ('c').get Char
--- #eval Environment.get ('c' *: "a" *: 1) Char
--- #eval Environment.get ('c' *: "a" *: 1 *: "b") String
--- #eval Environment.get ('c' *: "a" *: 1) Nat
-
--- #check_failure Environment.get ('c' *: "a" *: 1) Unit
-
-
 namespace EnvExamples
-
   open Environment
+
+
+  example : get 'c'               Char = 'c' := rfl
+  example : get ('c', "a", 1) Char = 'c' := rfl
+  example : get ('c', "a", 1)  Nat = 1   := rfl
+  example : get ('c', "a", 1) Unit = ()  := rfl
+
+  example : get ('c', "a", 1, "b") String = "a" := rfl
+
+  #check_failure get ('c', "a", 1) Int
+
+  -- Order does not matter
+  example : get ('c', "a", 1, "b") (String × Nat) = ("a", 1) := rfl
+  example : get ('c', "a", 1, "b") (Nat × String) = (1, "a") := rfl
+
+  -- Note that only the first String "a" is picked up.
+  example : get ('c', "a", 1, "b") (Char × String) = ('c', "a") := rfl
 
   -- Make it a Type 1 on purpose to verify that an Environment can hold types on different universes
 
@@ -153,21 +148,16 @@ namespace EnvExamples
   def p := Point.mk 1 2
 
 
-
   def e0: EmptyEnv                     := empty
   def e1: Environment String           := e0.add "<secret>"
   def e2: Environment (Point × String) := e1.add p
 
-  -- #check_failure e0.get Unit
 
-  -- #check_failure e1.get Unit
   example : e1.get String = "<secret>" := rfl
-
-  -- #check_failure e2.get Unit
   example : e2.get String = "<secret>" := rfl
   example : e2.get Point  = p          := rfl
   
-  -- #check_failure e2.get Int
+  #check_failure e2.get Int
 
 end EnvExamples
 
