Z/Core.lean
@@ -4,7 +4,6 @@ import Z.InterruptStatus
 import Z.Environment
 import Z.Metadata
 
-
 /-- Z R E A  -/
 inductive Z : Type -> Type -> Type -> Type 1 where
   | private internal.done (exit : Exit E A) (md := mempty) : Z R E A 
